test/artifact/hacl-star/pneutube/SocketIO.fst
@@ -20,9 +20,12 @@ assume val socket_rgn: r:rid{is_eternal_region r /\ file_rgn <> r}
 type socket_ref = sb:buffer socket{length sb = 1 /\ socket_rgn = (frameOf sb)}
 
 (* The socket state only depends on the socket region *)
-assume val current_state_: FStar.Heap.heap -> socket -> GTot socket_state
-val current_state: FStar.HyperStack.mem -> socket -> GTot socket_state
-let current_state h s = current_state_ (Map.sel h.h socket_rgn) s
+(* assume val current_state_: FStar.Heap.heap -> socket -> GTot socket_state *)
+(* val current_state: FStar.HyperStack.mem -> socket -> GTot socket_state *)
+(* let current_state h s = current_state_ (Map.sel h.h socket_rgn) s *)
+assume val current_state_: socket -> GTot socket_state
+val current_state: h:FStar.HyperStack.mem -> s:socket_ref{live h s}  -> GTot socket_state
+let current_state h s = current_state_ (get h s 0)
 
 
 assume val tcp_connect:
@@ -35,7 +38,7 @@ assume val tcp_connect:
       HS.modifies (Set.singleton socket_rgn) h0 h1
       /\ modifies_buf_1 socket_rgn s h0 h1 (* When connecting the socket reference was modified *)
       /\ live h1 s /\ live h1 host
-      /\ (match r with | SocketOk -> let sh = get h1 s 0 in current_state h1 sh = Open
+      /\ (match r with | SocketOk -> current_state h1 s = Open
                       | _ -> True)))
 
 assume val tcp_listen: port:u32 -> s:socket_ref -> ST sresult
@@ -44,17 +47,16 @@ assume val tcp_listen: port:u32 -> s:socket_ref -> ST sresult
       HS.modifies (Set.singleton socket_rgn) h0 h1
       /\ modifies_buf_1 socket_rgn s h0 h1 (* When connecting the socket reference was modified *)
       /\ live h1 s
-      /\ (match r with | SocketOk -> let sh = get h1 s 0 in current_state h1 sh = Open
+      /\ (match r with | SocketOk -> current_state h1 s = Open
                       | _ -> True)))
 
 
 assume val tcp_accept: l:socket_ref -> s:socket_ref{disjoint l s} -> ST sresult
-    (requires (fun h -> live h s /\ live h l /\ current_state h (get h l 0) = Open))
+    (requires (fun h -> live h s /\ live h l /\ current_state h l = Open))
     (ensures  (fun h0 r h1 -> live h1 s /\ live h1 l
       /\ HS.modifies (Set.singleton socket_rgn) h0 h1
       /\ modifies_buf_1 socket_rgn s h0 h1
-      /\ (match r with | SocketOk -> (let sh = get h1 s 0 in current_state h1 sh = Open
-                                     /\ current_state h1 (get h1 l 0) = Open)
+      /\ (match r with | SocketOk -> (current_state h1 s = Open /\ current_state h1 l = Open)
                       | _ -> True)))
 
 
@@ -62,12 +64,13 @@ assume val tcp_write_all: s:socket_ref ->
   b:uint8_p ->
   len:u64{U64.v len <= length b} ->
   Stack sresult
-    (requires (fun h0 -> live h0 s /\ live h0 b /\ current_state h0 (get h0 s 0) = Open))
+    (requires (fun h0 -> live h0 s /\ live h0 b /\ current_state h0 s = Open))
     (ensures  (fun h0 r h1 -> live h1 s /\ live h1 b
-      /\ h0 == h1 // JK: assuming that nothing changes for simplicity
+      /\ HS.modifies (Set.singleton socket_rgn) h0 h1
+      /\ modifies_buf_1 socket_rgn s h0 h1
       (* /\ HS.modifies (Set.singleton socket_rgn) h0 h1 *)
       (* /\ HS.modifies_ref socket_rgn !{} h0 h1 *)
-      /\ (r = SocketOk ==> current_state h1 (get h1 s 0) = Open)))
+      /\ (r = SocketOk ==> current_state h1 s = Open)))
 
 
 assume val tcp_read_all:
@@ -75,9 +78,11 @@ assume val tcp_read_all:
   b:buffer u8{frameOf b <> socket_rgn} ->
   len:u64{length b >= U64.v len} ->
   Stack sresult
-    (requires (fun h0 -> live h0 s /\ live h0 b /\ current_state h0 (get h0 s 0) = Open))
-    (ensures  (fun h0 r h1 -> live h1 s /\ live h1 b /\ modifies_1 b h0 h1
-      /\ (r = SocketOk ==> current_state h1 (get h1 s 0) = Open)))
+    (requires (fun h0 -> live h0 s /\ live h0 b /\ current_state h0 s = Open))
+    (ensures  (fun h0 r h1 -> live h1 s /\ live h1 b
+      /\ modifies_buf_1 (frameOf b) b h0 h1
+      /\ HS.modifies (Set.singleton (frameOf b)) h0 h1
+      /\ (r = SocketOk ==> current_state h1 s = Open)))
 
 
 assume val tcp_close: s:socket_ref -> ST sresult
@@ -85,4 +90,4 @@ assume val tcp_close: s:socket_ref -> ST sresult
     (ensures  (fun h0 r h1 -> live h1 s
       /\ HS.modifies (Set.singleton socket_rgn) h0 h1
       /\ modifies_buf_1 socket_rgn s h0 h1
-      /\ (r = SocketOk ==> current_state h1 (get h1 s 0) = Closed)))
+      /\ (r = SocketOk ==> current_state h1 s = Closed)))
